added KILL evidence extension alternative to drop ASP evidence results and clear the CVM bundle

src/Appraisal_Evidence.v
@@ -59,6 +59,7 @@ Fixpoint encodeEv (e:EvidenceC) : RawEv :=
   | ggc _ _ bs e' => bs :: (encodeEv e')
   | hhc _ _ bs _ => [bs]
   | eec _ _ bs _ => [bs]
+  | kkc _ _ _ => []
   | ssc e1 e2 => (encodeEv e1) ++ (encodeEv e2)
   end.
 
@@ -86,7 +87,13 @@ Fixpoint reconstruct_ev' (ls:RawEv) (et:Evidence) : Opt EvidenceC :=
       match ls' with
       | [] => Some (eec p ps bs et')
       | _ => None
-      end 
+      end
+    | KILL =>
+      (* '(bs, ls') <- peel_bs ls ;; *)
+      match ls with
+      | [] => Some (kkc p ps et')
+      | _ => None
+      end
     end
       (*
   | gg p ps et' =>
