src/Example_Phrases_Demo.v
@@ -15,15 +15,15 @@ Definition term1 := att 1 (asp SIG).
 
 Definition create_and_load_ak : Term :=
   asp (
-  ASPC ALL COMP (asp_paramsC cal_ak_aspid cal_ak_args source_plc cal_ak_targid)).
+  ASPC ALL EXTD (asp_paramsC cal_ak_aspid cal_ak_args source_plc cal_ak_targid)).
 
 Definition pub_key_to_bc : Term :=
   asp (
-  ASPC ALL COMP (asp_paramsC pub_bc_aspid pub_bc_args source_plc pub_bc_targid)).
+  ASPC ALL EXTD (asp_paramsC pub_bc_aspid pub_bc_args source_plc pub_bc_targid)).
 
 Definition get_data : Term :=
   asp (
-  ASPC ALL COMP (asp_paramsC get_data_aspid get_data_args source_plc get_data_targid)).
+  ASPC ALL EXTD (asp_paramsC get_data_aspid get_data_args source_plc get_data_targid)).
 
 Definition tpm_sig : Term :=
   asp (
@@ -31,13 +31,17 @@ Definition tpm_sig : Term :=
 
 Definition ssl_enc : Term :=
   asp (
-  ASPC ALL ENCR (asp_paramsC ssl_enc_aspid ssl_enc_args source_plc ssl_enc_targid)).
+      ASPC ALL EXTD (asp_paramsC ssl_enc_aspid ssl_enc_args source_plc ssl_enc_targid)).
+
+Definition local_enc : Term :=
+  asp (ENC 0).
 
 Definition demo_phrase : Term :=
   <{ create_and_load_ak ->
      pub_key_to_bc ->
      get_data ->
      tpm_sig ->
+     (*local_enc*)
      ssl_enc }>.
 
 
