src/Term_Defs_Core.v
@@ -60,7 +60,8 @@ Inductive ASP_PARAMS: Set :=
 Inductive FWD: Set :=
 | COMP
 | ENCR
-| EXTD.
+| EXTD
+| KILL.
 
 (** The structure of evidence. *)
 Inductive Evidence: Set :=
@@ -124,6 +125,7 @@ Notation "x -> y" := (lseq x y) (in custom copland_entry at level 99, right asso
 Notation "!" := (asp SIG) (in custom copland_entry at level 98).
 Notation "#" := (asp HSH) (in custom copland_entry at level 98).
 Notation "* p" := (asp (ENC p)) (in custom copland_entry at level 98).
+Notation "$" := (asp KILL) (in custom copland_entry at level 98).
 Notation "'__'" := (asp CPY) (in custom copland_entry at level 98).
 Notation "'{}'" := (asp NULL) (in custom copland_entry at level 98).
 Notation "'<<' x y z '>>'" := (asp (ASPC ALL EXTD (asp_paramsC x nil y z))) 
